General cleanup.

examples/plain/Context.v
@@ -1,11 +1,12 @@
+(** * Context *)
 Require Import Omega List Program.Equality.
 Require Import Autosubst.
 
-Fixpoint atn {X} l n (x : X) := 
-  match l with 
+Fixpoint atn {X} l n (x : X) :=
+  match l with
     | nil => False
-    | y :: l' => match n with 
-                  | 0 => x = y 
+    | y :: l' => match n with
+                  | 0 => x = y
                   | S n' => atn l' n' x
                 end
   end.
@@ -14,34 +15,37 @@ Fixpoint atn {X} l n (x : X) :=
 Section SubstInstance.
 
 Context {term : Type}.
-Context {Ids_term : Ids term} {Rename_term : Rename term} {Subst_term : Subst term}.
-Context {subst_lemmas : SubstLemmas term}.
+Context {Ids_term : Ids term} {Rename_term : Rename term}
+  {Subst_term : Subst term} {SubstLemmas_term : SubstLemmas term}.
 
 Inductive atnd: list term -> var -> term -> Prop :=
-| Atnd0 Delta A A': A' = A.[ren(+1)] -> atnd (A :: Delta) 0 A'
-| AtndS Delta x A B B' : atnd Delta x B -> B' = B.[ren(+1)] -> atnd (A :: Delta) (S x) B'
-.
+| Atnd0 Delta A A' :
+    A' = A.[ren(+1)] -> atnd (A :: Delta) 0 A'
+| AtndS Delta x A B B' :
+    atnd Delta x B -> B' = B.[ren(+1)] -> atnd (A :: Delta) (S x) B'.
 
-Lemma atn_mmap {f : term -> term} {Gamma x A A'} : atn Gamma x A -> A' = (f A) -> atn (mmap f Gamma) x A'.
+Lemma atn_mmap {f : term -> term} {Gamma x A A'} :
+  atn Gamma x A -> A' = (f A) -> atn (mmap f Gamma) x A'.
 Proof.
   revert x.
   induction Gamma; intros; simpl in *; trivial.
   destruct x; subst; eauto.
 Qed.
 
-Lemma mmap_atn {f : term -> term} {Gamma x A'} : atn (mmap f Gamma) x A' -> exists A, A' = (f A) /\ atn Gamma x A.
+Lemma mmap_atn {f : term -> term} {Gamma x A'} :
+  atn (mmap f Gamma) x A' -> exists A, A' = (f A) /\ atn Gamma x A.
 Proof.
-  revert x. induction Gamma; intros; simpl in *. 
+  revert x. induction Gamma; intros; simpl in *.
   - contradiction.
   - destruct x; subst; eauto.
 Qed.
 
-Lemma up_mmap_atn zeta xi Gamma1 Gamma2 A x: 
+Lemma up_mmap_atn zeta xi Gamma1 Gamma2 A x :
   (forall x B, atn Gamma1 x B -> atn Gamma2 (zeta x) B.[ren xi]) ->
   atn (mmap (subst (ren (+1))) Gamma1) x A ->
   atn (mmap (subst (ren (+1))) Gamma2) (zeta x) A.[ren (0 .: xi >>> (+1))].
 Proof.
-  intros H1 H2. 
+  intros H1 H2.
   edestruct (mmap_atn H2) as [? [? ?]]. subst.
   eapply atn_mmap; eauto. autosubst.
 Qed.
@@ -54,21 +58,26 @@ Proof.
   intros H1 H2; destruct x; simpl; inv H2; econstructor; eauto; autosubst.
 Qed.
 
-Lemma atnd_steps x Gamma Delta A : atnd Gamma x A <-> atnd (Delta ++ Gamma) (length Delta + x) A.[ren(+(length Delta))].
+Lemma atnd_steps x Gamma Delta A :
+  atnd Gamma x A <->
+  atnd (Delta ++ Gamma) (length Delta + x) A.[ren(+(length Delta))].
 Proof.
   revert A x.
   induction Delta; intros.
-  - split. 
+  - split.
     + autosubst.
     + autosubst.
-  - simpl. cutrewrite (A.[ren (+S (length Delta))] = A.[ren(+length Delta)].[ren(+1)]); [idtac|autosubst].
+  - simpl. cutrewrite (A.[ren (+S (length Delta))] =
+                       A.[ren(+length Delta)].[ren(+1)]); [idtac|autosubst].
     split.
       + econstructor. eapply IHDelta; eassumption. reflexivity.
-      + intros H. inv H. rewrite IHDelta. apply lift_inj in H5. subst. eassumption.
+      + intros H. inv H. rewrite IHDelta. apply lift_inj in H5.
+        subst. eassumption.
 Qed.
 
-Lemma atnd_steps' x Gamma Delta A :  atnd (Delta ++ Gamma) (x + length Delta) A ->
-                               exists B, A = B.[ren(+(length Delta))] /\ atnd Gamma x B.
+Lemma atnd_steps' x Gamma Delta A :
+  atnd (Delta ++ Gamma) (x + length Delta) A ->
+  exists B, A = B.[ren(+(length Delta))] /\ atnd Gamma x B.
 Proof.
   revert A x.
   induction Delta; intros.
@@ -82,26 +91,27 @@ Proof.
     intuition autosubst.
 Qed.
 
-Corollary atnd_step Delta A x B : atnd Delta x A <-> atnd (B :: Delta) (S x) A.[ren(+1)].
+Corollary atnd_step Delta A x B :
+  atnd Delta x A <-> atnd (B :: Delta) (S x) A.[ren(+1)].
 Proof.
   apply atnd_steps with (Delta := B :: nil).
 Qed.
 
-Lemma atnd_repl Gamma A Delta : 
+Lemma atnd_repl Gamma A Delta :
   (atnd (Delta ++ A :: Gamma) (length Delta) A.[ren(+ S (length Delta))]) /\
-  (forall x B A', x <> length Delta -> atnd (Delta ++ A :: Gamma) x B -> atnd (Delta ++ A' :: Gamma) x B).
+  (forall x B A',
+     x <> length Delta -> atnd (Delta ++ A :: Gamma) x B ->
+     atnd (Delta ++ A' :: Gamma) x B).
 Proof.
   split.
-  - pose proof (atnd_steps 0 (A :: Gamma) Delta A.[ren(+1)]) as H.
-    rewrite plus_0_r in H.
-    cutrewrite (A.[ren (+1)].[ren (+length Delta)] =  A.[ren (+S (length Delta))]) in H. { apply H. now constructor. }
-    autosubst.
+  - pose proof (atnd_steps 0 (A :: Gamma) Delta A.[ren(+1)]) as H. asimpl in H.
+    apply H. now constructor.
   - intros x. revert Gamma A Delta.
     induction x; intros Gamma A Delta H B A' H_atn.
     + destruct Delta as [| C Delta]. { now intuition. }
       simpl in *.
-      inv H_atn. now constructor. 
-    + destruct Delta as [| C Delta]; simpl in *. 
+      inv H_atn. now constructor.
+    + destruct Delta as [| C Delta]; simpl in *.
       * inv H_atn. econstructor. eassumption. reflexivity.
       * inv H_atn. econstructor. eapply IHx; eauto. reflexivity.
 Qed.
@@ -111,10 +121,14 @@ Proof.
   revert x. induction Delta; intuition; asimpl in *; ainv.
   - destruct x. omega. cut(x < length Delta). omega.
     ainv. firstorder.
-  - destruct x. 
-    + eexists. now econstructor. 
+  - destruct x.
+    + eexists. now econstructor.
     + edestruct IHDelta as [_ [? ?]]. cut(x < length Delta); eauto. omega.
       eexists. econstructor; eauto.
 Qed.
 
 End SubstInstance.
+
+(* Local Variables: *)
+(* coq-load-path: (("." "Plain")) *)
+(* End: *)
