theories/Autosubst.v
@@ -5,3 +5,7 @@ Require Export Autosubst_Tactics.
 Require Export Autosubst_Lemmas.
 Require Export Autosubst_Derive.
 Require Export Autosubst_MMapInstances.
+
+(* Local Variables: *)
+(* coq-load-path: (("." "Autosubst")) *)
+(* End: *)
